eliminated global SIMPSET, CLASET etc. -- refer to explicit context;

doc-src/TutorialI/Protocol/Message.thy
@@ -1,5 +1,4 @@
 (*  Title:      HOL/Auth/Message
-    ID:         $Id$
     Author:     Lawrence C Paulson, Cambridge University Computer Laboratory
     Copyright   1996  University of Cambridge
 
@@ -830,9 +829,9 @@ val pushes = thms "pushes";
 (*Prove base case (subgoal i) and simplify others.  A typical base case
   concerns  Crypt K X \<notin> Key`shrK`bad  and cannot be proved by rewriting
   alone.*)
-fun prove_simple_subgoals_tac i = 
-    force_tac (claset(), simpset() addsimps [@{thm image_eq_UN}]) i THEN
-    ALLGOALS Asm_simp_tac
+fun prove_simple_subgoals_tac (cs, ss) i = 
+    force_tac (cs, ss addsimps [@{thm image_eq_UN}]) i THEN
+    ALLGOALS (asm_simp_tac ss)
 
 (*Analysis of Fake cases.  Also works for messages that forward unknown parts,
   but this application is no longer necessary if analz_insert_eq is used.
@@ -857,8 +856,7 @@ fun atomic_spy_analz_tac (cs,ss) = SELECT_GOAL
 		  (cs addIs [analz_insertI,
 				   impOfSubs analz_subset_parts]) 4 1))
 
-(*The explicit claset and simpset arguments help it work with Isar*)
-fun gen_spy_analz_tac (cs,ss) i =
+fun spy_analz_tac (cs,ss) i =
   DETERM
    (SELECT_GOAL
      (EVERY 
@@ -870,8 +868,6 @@ fun gen_spy_analz_tac (cs,ss) i =
        simp_tac ss 1,
        REPEAT (FIRSTGOAL (resolve_tac [allI,impI,notI,conjI,iffI])),
        DEPTH_SOLVE (atomic_spy_analz_tac (cs,ss) 1)]) i)
-
-fun spy_analz_tac i = gen_spy_analz_tac (claset(), simpset()) i
 *}
 
 text{*By default only @{text o_apply} is built-in.  But in the presence of
@@ -919,7 +915,7 @@ done
 lemmas Fake_parts_sing_imp_Un = Fake_parts_sing [THEN [2] rev_subsetD]
 
 method_setup spy_analz = {*
-    Scan.succeed (SIMPLE_METHOD' o gen_spy_analz_tac o local_clasimpset_of) *}
+    Scan.succeed (SIMPLE_METHOD' o spy_analz_tac o local_clasimpset_of) *}
     "for proving the Fake case when analz is involved"
 
 method_setup atomic_spy_analz = {*
