src/HOL/SET-Protocol/MessageSET.thy
@@ -1,5 +1,4 @@
 (*  Title:      HOL/Auth/SET/MessageSET
-    ID:         $Id$
     Authors:     Giampaolo Bella, Fabio Massacci, Lawrence C Paulson
 *)
 
@@ -846,9 +845,9 @@ struct
 (*Prove base case (subgoal i) and simplify others.  A typical base case
   concerns  Crypt K X \<notin> Key`shrK`bad  and cannot be proved by rewriting
   alone.*)
-fun prove_simple_subgoals_tac i =
-    CLASIMPSET' (fn (cs, ss) => force_tac (cs, ss addsimps [@{thm image_eq_UN}])) i THEN
-    ALLGOALS (SIMPSET' asm_simp_tac)
+fun prove_simple_subgoals_tac (cs, ss) i =
+    force_tac (cs, ss addsimps [@{thm image_eq_UN}]) i THEN
+    ALLGOALS (asm_simp_tac ss)
 
 (*Analysis of Fake cases.  Also works for messages that forward unknown parts,
   but this application is no longer necessary if analz_insert_eq is used.
@@ -873,8 +872,7 @@ fun atomic_spy_analz_tac (cs,ss) = SELECT_GOAL
 		  (cs addIs [@{thm analz_insertI},
 				   impOfSubs @{thm analz_subset_parts}]) 4 1))
 
-(*The explicit claset and simpset arguments help it work with Isar*)
-fun gen_spy_analz_tac (cs,ss) i =
+fun spy_analz_tac (cs,ss) i =
   DETERM
    (SELECT_GOAL
      (EVERY
@@ -886,8 +884,6 @@ fun gen_spy_analz_tac (cs,ss) i =
        simp_tac ss 1,
        REPEAT (FIRSTGOAL (resolve_tac [allI,impI,notI,conjI,iffI])),
        DEPTH_SOLVE (atomic_spy_analz_tac (cs,ss) 1)]) i)
-
-val spy_analz_tac = CLASIMPSET' gen_spy_analz_tac;
 
 end
 *}
@@ -941,7 +937,7 @@ lemmas Fake_parts_sing_imp_Un = Fake_parts_sing [THEN [2] rev_subsetD]
 
 method_setup spy_analz = {*
     Scan.succeed (fn ctxt =>
-        SIMPLE_METHOD' (MessageSET.gen_spy_analz_tac (local_clasimpset_of ctxt))) *}
+        SIMPLE_METHOD' (MessageSET.spy_analz_tac (local_clasimpset_of ctxt))) *}
     "for proving the Fake case when analz is involved"
 
 method_setup atomic_spy_analz = {*
